\documentclass{article}
\usepackage[utf8]{inputenc}
\usepackage{amsmath}

\title{Applied Math HW}
\author{Rodolfo Lopez}
\date{February 2023}

\begin{document}

\maketitle

\section{Problem}
Find the general solution to $y' + 15t^{14}y = t^{15}.$
Use the variable $I = \int e^{t^{15}}dt$ where it occurs in your answer since this integral is not easily computable. Note that the arbitrary constant $C$ would come from actually computing the integral $I$, so you do not need to write it. 

\subsection{Step 1}
We will find an appropriate integrating factor $\mu(t)$. Multiply both sides of the equation by that factor, and express the left side as the derivative of a product. 


\begin{align} 
    \mu(t) 
    &= e^{\int15t^{14}dt} \\
    &= e^{t^{15}} 
\end{align}


\begin{align}
    y' + 15t^{14}y &= t^{15}  \\
    \implies y'e^{t^{15}} + 15t^{14}e^{t^{15}} &= t^{15}e^{t^{15}} \\
    \implies \frac{d}{dt}[e^{t^{15}}y] &= t^{15}e^{t^{15}}.
\end{align}

\subsection{Step 2}
We will use integration by parts to find the solution for the differential equation.

\begin{align}
    \implies e^{t^{15}}y &= \int t^{15}e^{t^{15}}dt\\
    \implies e^{t^{15}}y &= \int t t^{14} e^{t^{15}} dt\\
    \implies e^{t^{15}}y &= \frac{t}{15}e^{t^{15}}-\frac{1}{15}\int e^{t^{15}} dt\\
    \implies e^{t^{15}}y &= \frac{t}{15}e^{t^{15}} - \frac{I}{15}.
\end{align}

So we finally have

\begin{align}
    y &= \frac{t}{15} - \frac{I}{15}e^{-t^{15}}.
\end{align}

\end{document}
